@prefix : <http://www.example.org/lemon/morph#> .
@prefix owl: <http://www.w3.org/2002/07/owl#> .
@prefix rdf: <http://www.w3.org/1999/02/22-rdf-syntax-ns#> .
@prefix xml: <http://www.w3.org/XML/1998/namespace> .
@prefix xsd: <http://www.w3.org/2001/XMLSchema#> .
@prefix rdfs: <http://www.w3.org/2000/01/rdf-schema#> .

<http://www.example.org/lemon/morph#> a owl:Ontology ;
	owl:imports <http://www.w3.org/ns/lemon/decomp> , <http://www.w3.org/ns/lemon/ontolex> , <http://www.w3.org/ns/lemon/vartrans> .
# 
# 
# #################################################################
# #
# #    Object Properties
# #
# #################################################################
# 
# 
# http://www.example.org/lemon/morph#belongsToMorphPattern

:belongsToMorphPattern a owl:ObjectProperty ;
	rdfs:domain :InflectionalParadigm ;
	rdfs:range :MorphologicalPattern ;
	rdfs:comment "This property assigns an inflectional pattern of a form as belonging to a morphological pattern of a lexical entry."@en ;
	rdfs:label "belongs to morphological pattern"@en .
# 
# http://www.example.org/lemon/morph#consistsOf

:consistsOf a owl:ObjectProperty ;
	rdfs:domain <http://www.w3.org/ns/lemon/ontolex#Form> ;
	rdfs:range :Morph ;
	rdfs:comment "This property states into which Morph resources a Form resource can be segmented."@en ;
	rdfs:label "consists of"@en .
# 
# http://www.example.org/lemon/morph#derivationalRel

:derivationalRel a owl:ObjectProperty ;
	rdfs:subPropertyOf <http://www.w3.org/ns/lemon/vartrans#lexicalRel> ;
	rdfs:comment "The 'derivationalRel' property relates two lexical entries that stand in some derivational relation."@en .
# 
# http://www.example.org/lemon/morph#grammaticalMeaning

:grammaticalMeaning a owl:ObjectProperty ;
	rdfs:domain :Morph ;
	rdfs:comment "This property assigns a grammatical meaning to a morph resource."@en ;
	rdfs:label "grammatical meaning"@en .
# 
# http://www.example.org/lemon/morph#hasMorphStatus

:hasMorphStatus a owl:ObjectProperty , owl:FunctionalProperty ;
	rdfs:domain :Morph , <http://www.w3.org/ns/lemon/ontolex#Affix> ;
	rdfs:range :MorphValue ;
	rdfs:comment "States whether a morphological element functions as inflectional or derivational."@en ;
	rdfs:label "has morph status"@en .
# 
# http://www.example.org/lemon/morph#hasParadigm

:hasParadigm a owl:ObjectProperty ;
	rdfs:domain <http://www.w3.org/ns/lemon/ontolex#Form> ;
	rdfs:range :InflectionalParadigm ;
	rdfs:comment "This property assigns a form to an inflectional paradigm."@en ;
	rdfs:label "has paradigm"@en .
# 
# http://www.example.org/lemon/morph#meaning

:meaning a owl:ObjectProperty ;
	rdfs:domain :Morph ;
	rdfs:range <http://www.w3.org/ns/lemon/ontolex#LexicalSense> ;
	rdfs:comment "This property assigns a lexical sense to a morph resource."@en ;
	rdfs:label "meaning"@en .
# 
# http://www.w3.org/ns/lemon/ontolex#morphologicalPattern

<http://www.w3.org/ns/lemon/ontolex#morphologicalPattern> rdfs:range :MorphologicalPattern .
# 
# 
# 
# #################################################################
# #
# #    Classes
# #
# #################################################################
# 
# 
# http://www.example.org/lemon/morph#AffixMorph

:AffixMorph a owl:Class ;
	rdfs:subClassOf :Morph ;
	rdfs:comment "An affix is a bound segmental morph."@en ;
	rdfs:label "affix morph"@en .
# 
# http://www.example.org/lemon/morph#DerivationalRelation

:DerivationalRelation a owl:Class ;
	rdfs:subClassOf <http://www.w3.org/ns/lemon/vartrans#LexicalRelation> ;
	rdfs:comment "A 'derivational relation' is a lexical relation that relates two lexical entries by means of a derivational affix."@en .
# 
# http://www.example.org/lemon/morph#InflectionalParadigm

:InflectionalParadigm a owl:Class ;
	rdfs:comment "A structured set of inflected forms according to specific grammatical parameters."@en ;
	rdfs:label "inflectional paradigm"@en .
# 
# http://www.example.org/lemon/morph#Morph

:Morph a owl:Class ;
	owl:disjointWith <http://www.w3.org/ns/lemon/ontolex#LexicalEntry> ;
	rdfs:comment "A morph is a concrete primitive element of morphological analysis."@en ;
	rdfs:label "morph"@en .
# 
# http://www.example.org/lemon/morph#MorphValue

:MorphValue a owl:Class ;
	rdfs:comment "The value of a morph states the relationship that holds between the morph and the forms or lexical entries in which it can occur."@en ;
	rdfs:label "morph value"@en .
# 
# http://www.example.org/lemon/morph#MorphologicalPattern

:MorphologicalPattern a owl:Class ;
	rdfs:comment "The morphological pattern states the inflectional, derivational or compositional building pattern that applies to a lexical entry."@en ;
	rdfs:label "morphological pattern"@en .
# 
# http://www.example.org/lemon/morph#RootMorph

:RootMorph a owl:Class ;
	rdfs:subClassOf :Morph ;
	rdfs:comment "A morph that constitutes the semantic nucleus of a stem. It cannot be further segmented and is often not specified for a part of speech."@en ;
	rdfs:label "root morph"@en .
# 
# http://www.example.org/lemon/morph#SimulfixMorph

:SimulfixMorph a owl:Class ;
	rdfs:subClassOf :Morph ;
	rdfs:comment "A simulfix is a bound morph that entails a change or replacement of vowels or consonants (usually vowels) which changes the meaning of a word, e.g. \\\"eat\\\" in past tense becomes \\\"ate \\\"tooth\\\" becomes \\\"teeth\\\" when plural."@en ;
	rdfs:label "simulfix morph"@en .
# 
# http://www.example.org/lemon/morph#StemMorph

:StemMorph a owl:Class ;
	rdfs:subClassOf :Morph ;
	rdfs:comment "The stem is the morph to which inflectional marking applies."@en ;
	rdfs:label "stem morph"@en .
# 
# http://www.example.org/lemon/morph#TransfixMorph

:TransfixMorph a owl:Class ;
	rdfs:subClassOf :Morph ;
	rdfs:comment "A transfix is a discontinuous affix."@en ;
	rdfs:label "transfix morph"@en .
# 
# http://www.example.org/lemon/morph#ZeroMorph

:ZeroMorph a owl:Class ;
	rdfs:subClassOf :Morph ;
	rdfs:comment "A morphs that that corresponds to no overt form, i.e. orthographic or phonetic representation."@en ;
	rdfs:label "zero morph"@en .
# 
# http://www.w3.org/ns/lemon/ontolex#LexicalEntry
# 
# 
# 
# #################################################################
# #
# #    Individuals
# #
# #################################################################
# 
# 
# http://www.example.org/lemon/morph#derivational

:derivational a owl:NamedIndividual , :MorphValue .
# 
# http://www.example.org/lemon/morph#inflectional

:inflectional a owl:NamedIndividual , :MorphValue .
# 
# 
# 
# #################################################################
# #
# #    General axioms
# #
# #################################################################
# 
# 

_:genid1 a owl:AllDifferent ;
	owl:distinctMembers _:genid3 .

_:genid3 a rdf:List ;
	rdf:first :derivational ;
	rdf:rest _:genid2 .

_:genid2 a rdf:List ;
	rdf:first :inflectional ;
	rdf:rest rdf:nil .
# 
# Generated by the OWL API (version 4.2.5.20160517-0735) https://github.com/owlcs/owlapi
